Simple_Firewall/SimpleFw_Semantics.thy
@@ -1,4 +1,4 @@
-theory SimpleFwSyntax                                                                                                             
+theory SimpleFw_Semantics
 imports Main "../Bitmagic/IPv4Addr" "../Bitmagic/BitrangeLists" "../Output_Format/Negation_Type"
   "../Firewall_Common_Decision_State"
   "../Primitive_Matchers/Iface"
